thy/AbstractInterpretation.thy
@@ -39,11 +39,12 @@ lemma [simp]:
   done
 
 definition "ifexd_valid bdd e \<equiv> (case e of IFD _ t e \<Rightarrow> bdd_node_valid bdd t \<and> bdd_node_valid bdd e | _ \<Rightarrow> True)"
-definition "bdd_sane bdd \<equiv> pointermap_sane (dpm bdd)"
+
+definition "bdd_sane bdd \<equiv> pointermap_sane (dpm bdd) \<and> map_invar_impl Rmi (dcl bdd) bdd"
 
 lemma [simp,intro!]: "bdd_sane emptymi" 
 	unfolding emptymi_def bdd_sane_def bdd.simps 
-by simp
+by(simp add: map_invar_impl_def)
 
 lemma prod_split3: "P (case prod of (x, xa, xaa) \<Rightarrow> f x xa xaa) = (\<forall>x1 x2 x3. prod = (x1, x2, x3) \<longrightarrow> P (f x1 x2 x3))"
 by(simp split: prod.splits)
